Logic/Modal/Standard/Kripke/Soundness.lean
@@ -3,12 +3,49 @@ import Logic.Modal.Standard.Deduction
 
 namespace LO.Modal.Standard.Kripke
 
-variable {α : Type u}
-         {L : DeductionParameter α} [L.HasNecOnly]
+variable {α : Type u} {Ax : AxiomSet α}
 
 open Deduction
 open Formula
 
+open DeductionParameter (Normal)
+
+lemma sound [definability : Ax.DefinesKripkeFrameClass 𝔽] (d : (Normal Ax) ⊢! p) : 𝔽 ⊧ p := by
+  induction d using Deduction.inducition_with_nec! with
+  | hMaxm h =>
+    simp only [Set.mem_setOf_eq] at h;
+    rcases h with (hK | hR);
+    . exact (Semantics.RealizeSet.setOf_iff.mp valid_on_KripkeFrameClass.axiomK) _ hK;
+    . intro F hF;
+      exact Semantics.RealizeSet.setOf_iff.mp (definability.defines.mpr hF) _ hR;
+  | hMdp ihpq ihp => exact valid_on_KripkeFrameClass.mdp ihpq ihp;
+  | hNec ih => exact valid_on_KripkeFrameClass.nec ih;
+  | hDisj₃ =>
+    simp_all [valid_on_KripkeFrameClass, valid_on_KripkeFrame, valid_on_KripkeModel];
+    intros; rename_i hpr hqr hpq;
+    cases hpq with
+    | inl hp => exact hpr hp;
+    | inr hq => exact hqr hq;
+  | _ => simp_all [valid_on_KripkeFrameClass, valid_on_KripkeFrame, valid_on_KripkeModel];
+
+instance instSound [Ax.DefinesKripkeFrameClass 𝔽] : Sound (DeductionParameter.Normal Ax) 𝔽 := ⟨sound⟩
+
+instance : Sound 𝐊 (AllFrameClass α) := by
+  simpa [←Normal.isK] using (instSound (Ax := 𝗞) (𝔽 := AllFrameClass α));
+
+lemma unprovable_bot (𝔽 : FrameClass α) [Ax.DefinesKripkeFrameClass 𝔽] [nonempty : 𝔽.IsNonempty] : (Normal Ax) ⊬! ⊥ := by
+  by_contra hC;
+  obtain ⟨F, hF⟩ := nonempty.nonempty
+  simpa using sound hC F hF;
+
+lemma consistent (𝔽 : FrameClass α) [Ax.DefinesKripkeFrameClass 𝔽] [𝔽.IsNonempty] : System.Consistent (Normal Ax) := by
+  apply System.Consistent.of_unprovable;
+  exact unprovable_bot 𝔽;
+
+instance : System.Consistent (𝐊 : DeductionParameter α) := by
+  simpa [←Normal.isK] using consistent (Ax := 𝗞) (𝔽 := AllFrameClass α)
+
+/-
 lemma sound_on_frameclass (d : L ⊢ p) : 𝔽(Ax(L)) ⊧ p := by
   induction d using Deduction.inducition_with_nec with
   | hMaxm h => exact validOnAxiomSetFrameClass_axiom h;
@@ -45,5 +82,6 @@ lemma unprovable_bot_finite [ne : 𝔽ꟳ(Ax(L)).IsNonempty] : L ⊬! ⊥ := by
 instance Consistent_of_nonemptyFiniteFrameClass [𝔽ꟳ(Ax(L)).IsNonempty] : System.Consistent L := System.Consistent.of_unprovable $ unprovable_bot_finite
 
 instance : System.Consistent (𝐊 : DeductionParameter α) := inferInstance
+-/
 
 end LO.Modal.Standard.Kripke
