Logic/Modal/Standard/Maximal.lean
@@ -132,7 +132,7 @@ lemma iff_Triv_classical : 𝐓𝐫𝐢𝐯 ⊢! p ↔ 𝐂𝐥 ⊢! pᵀᴾ := 
   . intro h;
     induction h.some using Deduction.inducition_with_nec with
     | hMaxm a =>
-      rcases a with (hK | hT) | hTc;
+      rcases a with (hK | hT | hTc);
       . obtain ⟨_, _, e⟩ := hK; subst_vars; dsimp [Axioms.K, TrivTranslation, toPropFormula]; apply imp_id!;
       . obtain ⟨_, e⟩ := hT; subst_vars; dsimp [Axioms.T, TrivTranslation, toPropFormula]; apply imp_id!;
       . obtain ⟨_, e⟩ := hTc; subst_vars; dsimp [Axioms.Tc, TrivTranslation, toPropFormula]; apply imp_id!;
